ref_impl/src/verifier/fstar_files/bosqueTypes.fst
@@ -38,10 +38,9 @@ type bosqueType =
 | BKeyedType
 | BErrorType
 | BListType : bosqueType -> bosqueType// User-defined types
+| BnSMain__Bar3Type
 | BnSMain__Bar2Type
 | BnSMain__Baz2Type
-| BnSMain__Bar3Type
-| BnSMain__Baz3Type
 | BnSMain__MusicianType
 | BnSMain__ArtistType
 | BnSMain__PlayerMarkType
@@ -70,6 +69,7 @@ let rec eqTypeList x y = match x with
 
 (* Definition to encode the subtype relation on Bosque types 
    i.e.forall x y.subtypeOf x y <===> x :> y *) 
+val subtypeOfList: x: list bosqueType -> list bosqueType -> Tot bool(decreases x)
 val subtypeOfSeq: n: nat -> x: sequence bosqueType n -> sequence bosqueType n -> Tot bool(decreases x) 
 val subtypeOf: x: bosqueType -> bosqueType -> Tot bool(decreases x) 
 let rec subtypeOf x y = match x, y with
@@ -115,19 +115,17 @@ let rec subtypeOf x y = match x, y with
 | BListType t1 , BListType t2 -> subtypeOf t1 t2
 // User-defined types
 // Reflexivity relation
+| BnSMain__Bar3Type, BnSMain__Bar3Type -> true
 | BnSMain__Bar2Type, BnSMain__Bar2Type -> true
 | BnSMain__Baz2Type, BnSMain__Baz2Type -> true
-| BnSMain__Bar3Type, BnSMain__Bar3Type -> true
-| BnSMain__Baz3Type, BnSMain__Baz3Type -> true
 | BnSMain__MusicianType, BnSMain__MusicianType -> true
 | BnSMain__ArtistType, BnSMain__ArtistType -> true
 | BnSMain__PlayerMarkType, BnSMain__PlayerMarkType -> true
 // Provide relation
-| BnSMain__Bar2Type, BnSMain__Baz2Type -> true
-| BObjectType, BnSMain__Bar2Type -> true
-| BObjectType, BnSMain__Bar3Type -> true
-| BnSMain__Baz2Type, BnSMain__Baz3Type -> true
 | BnSMain__Bar3Type, BnSMain__Baz2Type -> true
+| BObjectType, BnSMain__Bar3Type -> true
+| BObjectType, BnSMain__Bar2Type -> true
+| BnSMain__Bar2Type, BnSMain__Baz2Type -> true
 | BParsableType, BnSMain__MusicianType -> true
 | BParsableType, BnSMain__ArtistType -> true
 | BParsableType, BnSMain__PlayerMarkType -> true
