ref_impl/src/verifier/fstar_files/NSMain__main_main.fst
@@ -1,51 +1,30 @@
 module NSMain__main_main
+
 open Sequence
+open List
 open BosqueTypes
 open BosqueTerms
 open Util
 
 (* Type names *)
 let bTypedStringType_BAnyType = (BTypedStringType BAnyType)
-let bRecordType_3BBoolType_BIntType_bTypedStringType_BAnyTypefalse = BRecordType false 3 (SCons "f" 2 (SCons "g" 1 (SCons "h" 0 SNil))) (SCons BBoolType 2 (SCons BIntType 1 (SCons bTypedStringType_BAnyType 0 SNil)))
-let bRecordType_2BBoolType_BIntTypefalse = BRecordType false 2 (SCons "f" 1 (SCons "g" 0 SNil)) (SCons BBoolType 1 (SCons BIntType 0 SNil))
-let bRecordType_2BIntType_BBoolTypefalse = BRecordType false 2 (SCons "f" 1 (SCons "k" 0 SNil)) (SCons BIntType 1 (SCons BBoolType 0 SNil))
 
 (* Constant Declarations *)
 
 (* Function Declarations *)
 val nSMain__main : (x:bosqueTerm{subtypeOf BIntType (getType x)})
 let nSMain__main  = 
-  let __tmp_0 = (BRecord 3 (SCons "f" 2 (SCons "g" 1 (SCons "h" 0 SNil))) (SCons (BBool true) 2 (SCons (BInt 2) 1 (SCons (BTypedString "hello" BAnyType) 0 SNil)))) in
-  let xRecord = __tmp_0 in
-  let _ = assert_norm(subtypeOf bRecordType_3BBoolType_BIntType_bTypedStringType_BAnyTypefalse (getType xRecord)) in
-  let __tmp_6 = (nthRecord "g" 3 xRecord) in
-  let x_ProjectedRecord = __tmp_6 in
-  let __fresh_name1NSMain__main = (nthRecord "g" 3 xRecord) in
-  let __fresh_name0NSMain__main = (nthRecord "f" 3 xRecord) in
-  let __tmp_9 = (BRecord 2 (SCons "f" 1 (SCons "g" 0 SNil)) (SCons __fresh_name0NSMain__main 1 (SCons __fresh_name1NSMain__main 0 SNil))) in
-  let x = __tmp_9 in
-  let __tmp_10_arg_3 = (BBool false) in
-  let __tmp_10_arg_2 = (BBool true) in
-  let __tmp_10_arg_1 = (BInt 2) in
-  let __tmp_10_arg_0 = (BInt 1) in
-  let _ = assert_norm(subtypeOf BBoolType (getType __tmp_10_arg_3)) in
-  let _ = assert_norm(subtypeOf BBoolType (getType __tmp_10_arg_2)) in
-  let _ = assert_norm(subtypeOf BIntType (getType __tmp_10_arg_1)) in
-  let _ = assert_norm(subtypeOf BIntType (getType __tmp_10_arg_0)) in
-  let __tmp_10 = (BnSMain__Baz3 __tmp_10_arg_0 __tmp_10_arg_1 __tmp_10_arg_2 __tmp_10_arg_3) in
-  let e = __tmp_10 in
-  let _ = assert_norm(subtypeOf BnSMain__Baz3Type (getType e)) in
-  let __tmp_17 = (projectBnSMain__Baz3_f e) in
-  let e2 = __tmp_17 in
-  let __fresh_name1NSMain__main = (projectBnSMain__Baz3_k e) in
-  let __fresh_name0NSMain__main = (projectBnSMain__Baz3_f e) in
-  let __tmp_20 = (BRecord 2 (SCons "f" 1 (SCons "k" 0 SNil)) (SCons __fresh_name0NSMain__main 1 (SCons __fresh_name1NSMain__main 0 SNil))) in
-  let e3 = __tmp_20 in
+  let __tmp_0_arg_2 = (BBool true) in
+  let __tmp_0_arg_1 = (BInt 2) in
+  let __tmp_0_arg_0 = (BInt 1) in
+  let _ = assert_norm(subtypeOf BBoolType (getType __tmp_0_arg_2)) in
+  let _ = assert_norm(subtypeOf BIntType (getType __tmp_0_arg_1)) in
+  let _ = assert_norm(subtypeOf BIntType (getType __tmp_0_arg_0)) in
+  let __tmp_0 = (BnSMain__Baz2 __tmp_0_arg_0 __tmp_0_arg_1 __tmp_0_arg_2) in
+  let e = __tmp_0 in
   let _MIRProjectFromTypeConcept = (BInt 0) in
-  let e4 = __tmp_23 in
-  let _ConstructorPrimaryCollectionSingletons = (BInt 0) in
-  let m_list = __tmp_24 in
-  let __ir_ret__ = e2 in
+  let e2 = __tmp_6 in
+  let __ir_ret__ = (BInt 0) in
   let _return_ = __ir_ret__ in
   _return_
 
