ref_impl/src/verifier/fstar_files/trigger_example.fst
@@ -1,0 +1,95 @@
+module Trigger_example
+
+type list 'a : Type = 
+| LNil 
+| LCons : hd : 'a -> tl : list 'a -> list 'a 
+
+val length : list 'a -> Tot int
+let rec length x = match x with
+| LNil -> 0
+| LCons _ tl -> 1 + length tl
+
+val filter : ('a -> bool) -> list 'a -> list 'a
+let rec filter p x = match x with
+| LNil -> LNil
+| LCons hd tl -> if (p hd) then LCons (hd) (filter p tl) else (filter p tl)
+
+val map : ('a -> 'b) -> list 'a -> list 'b
+let rec map f x = match x with
+| LNil -> LNil
+| LCons hd tl -> LCons (f hd) (map f tl)
+
+val length_is_always_positive : x : list 'a -> 
+  Lemma (requires True) (ensures length x >= 0)
+let rec length_is_always_positive x = match x with
+| LNil -> ()
+| LCons _ tl -> length_is_always_positive tl
+
+val filtered_lists_are_smaller : p : ('a -> bool) -> x : list 'a -> 
+  Lemma (requires True) (ensures length x >= length (filter p x))
+let rec filtered_lists_are_smaller p x = match x with
+| LNil -> ()
+| LCons hd tl -> filtered_lists_are_smaller p tl
+
+val map_preserves_length : f : ('a -> 'b) -> x : list 'a -> 
+  Lemma (requires True) (ensures length x = length (map f x))
+let rec map_preserves_length f x = match x with 
+| LNil -> ()
+| LCons hd tl -> map_preserves_length f tl
+
+// val length_is_always_positive : x : list 'a -> Lemma (requires True) (ensures length x >= 0) [SMTPat (length x)]
+// let rec length_is_always_positive x = match x with
+// | LNil -> ()
+// | LCons _ tl -> length_is_always_positive tl
+
+// val filtered_lists_are_smaller : 
+// p : ('a -> bool) -> x : list 'a -> Lemma (requires True) (ensures length x >= length (filter p x)) [SMTPat (filter p x)]
+// let rec filtered_lists_are_smaller p x = match x with
+// | LNil -> ()
+// | LCons hd tl -> filtered_lists_are_smaller p tl
+
+// val map_preserves_length : f : ('a -> 'b) -> x : list 'a -> 
+//   Lemma (requires True) (ensures length x = length (map f x)) [SMTPat (map f x)]
+// let rec map_preserves_length f x = match x with 
+// | LNil -> ()
+// | LCons hd tl -> map_preserves_length f tl
+
+val positive_fun : x : list 'a -> Tot nat
+let positive_fun x = length x
+
+val another_positive_fun : x : list nat -> Tot nat
+let another_positive_fun x = length x - (length (filter (fun (x : nat) -> x = 0) x))
+
+
+assume type t
+
+assume val (+): t -> t -> t
+
+assume val plus_associative: x:t -> y:t -> z:t -> Lemma
+  (requires True)
+  (ensures  (x + y) + z == x + (y + z))
+  [SMTPat ((x + y) + z)]
+
+irreducible let trigger (x:t) (y:t) = True
+
+val test: x:t -> y:t -> z:t -> Lemma
+  (requires forall (a:t) (b:t).{:pattern (trigger a b)} trigger a b /\ a + b == b + a)
+  (ensures  (x + y) + z == (z + y) + x)
+let test x y z = cut (trigger z y /\ trigger x (z + y))
+
+
+// assume type t
+
+// assume val (+): t -> t -> t
+
+// assume val plus_associative: x:t -> y:t -> z:t -> Lemma
+//   (requires True)
+//   (ensures  (x + y) + z == x + (y + z))
+//   [SMTPat ((x + y) + z)]
+
+// irreducible let trigger (x:t) (y:t) = True
+
+// val test: x:t -> y:t -> z:t -> Lemma
+//   (requires forall (a:t) (b:t).{:pattern (trigger a b)} trigger a b /\ a + b == b + a)
+//   (ensures  (x + y) + z == (z + y) + x)
+// let test x y z = cut (trigger z y /\ trigger x (z + y))
